ocaml/src/ConfigUtil.ml
@@ -93,7 +93,7 @@ let suffix_dnnrc_typed () = "_tdnnrc.txt"
 let suffix_dnnrcsexp () = "_dnnrc.sexp"
 let suffix_nnrs () = "_nnrs.txt"
 let suffix_nnrs_core () = "_nnrs_core.txt"
-let suffix_nnrc_imp () = "_nnrc_imp.txt"
+let suffix_nnrs_imp () = "_nnrs_imp.txt"
 let suffix_nnrcmr () = "_nnrcmr.txt"
 let suffix_nnrcmr_spark_rdd () = "_nnrcmr_spark_rdd.txt"
 let suffix_nnrcmr_spark_rddsexp () = "_nnrcmr_spark_rdd.sexp"
@@ -131,7 +131,7 @@ let suffix_of_language lang =
   | QcertCompiler.L_dnnrc_typed -> suffix_dnnrc_typed ()
   | QcertCompiler.L_nnrs -> suffix_nnrs ()
   | QcertCompiler.L_nnrs_core -> suffix_nnrs_core ()
-  | QcertCompiler.L_nnrc_imp -> suffix_nnrc_imp ()
+  | QcertCompiler.L_nnrs_imp -> suffix_nnrs_imp ()
   | QcertCompiler.L_nnrcmr -> suffix_nnrcmr ()
   | QcertCompiler.L_cldmr -> suffix_nnrcmr_cldmr ()
   | QcertCompiler.L_js_ast -> suffix_js_ast ()
