ocaml/src/QcertOut.ml
@@ -37,7 +37,7 @@ let output_query pconf q =
   | QcertCompiler.Q_nnrc q -> pretty_query pconf pretty_nnrc q
   | QcertCompiler.Q_nnrs q -> pretty_query pconf pretty_nnrs q
   | QcertCompiler.Q_nnrs_core q -> pretty_query pconf pretty_nnrs_core q
-  | QcertCompiler.Q_nnrc_imp q -> pretty_query pconf pretty_nnrc_imp q
+  | QcertCompiler.Q_nnrs_imp q -> pretty_query pconf pretty_nnrs_imp q
   | QcertCompiler.Q_nnrcmr q -> pretty_query pconf pretty_nnrcmr q
   | QcertCompiler.Q_cldmr q -> pretty_query pconf pretty_cldmr q
   | QcertCompiler.Q_dnnrc q -> pretty_query pconf pretty_dnnrc q
