coq/Compiler/Driver/CompEval.v
@@ -36,7 +36,7 @@ Require Import NRARuntime.
 Require Import NRAEnvRuntime.
 Require Import NNRCRuntime.
 Require Import NNRSRuntime.
-Require Import NNRCimpRuntime.
+Require Import NNRSimpRuntime.
 Require Import NNRCMRRuntime.
 Require Import CldMRRuntime.
 Require Import DNNRCRuntime.
@@ -125,9 +125,9 @@ Section CompEval.
     Definition eval_nnrs (q:nnrs) (cenv: bindings) : option data :=
       NNRSEval.nnrs_eval_top h cenv q.
 
-    (* Language: nnrc_imp *)
-    Definition eval_nnrc_imp (q:nnrc_imp) (cenv: bindings) : option data :=
-      NNRCimpEval.nnrc_imp_eval_top h cenv q.
+    (* Language: nnrs_imp *)
+    Definition eval_nnrs_imp (q:nnrs_imp) (cenv: bindings) : option data :=
+      NNRSimpEval.nnrs_imp_eval_top h cenv q.
 
     (* Language: nnrcmr *)
     Definition eval_nnrcmr (q:nnrcmr) (dcenv: dbindings) : option data :=
@@ -183,7 +183,7 @@ Section CompEval.
       | Q_nnrc q => lift_output (eval_nnrc q (lift_input ev_in))
       | Q_nnrs_core q => lift_output (eval_nnrs_core q (lift_input ev_in))
       | Q_nnrs q => lift_output (eval_nnrs q (lift_input ev_in))
-      | Q_nnrc_imp q => lift_output (eval_nnrc_imp q (lift_input ev_in))
+      | Q_nnrs_imp q => lift_output (eval_nnrs_imp q (lift_input ev_in))
       | Q_nnrcmr q => lift_output (eval_nnrcmr q ev_in) (* XXX Does not localize, keeps distributed information XXX *)
       | Q_cldmr q => lift_output (eval_cldmr q (lift_input ev_in))
       | Q_dnnrc q => lift_output (eval_dnnrc q ev_in) (* XXX Does not localize, keeps distributed information XXX *)
@@ -214,7 +214,7 @@ Section CompEval.
       | Q_nnrc _ => Ev_out_unsupported ("No debug evaluation support for "++(name_of_language (language_of_query q)))
       | Q_nnrs_core _ => Ev_out_unsupported ("No debug evaluation support for "++(name_of_language (language_of_query q)))
       | Q_nnrs _ => Ev_out_unsupported ("No debug evaluation support for "++(name_of_language (language_of_query q)))
-      | Q_nnrc_imp _ => Ev_out_unsupported ("No debug evaluation support for "++(name_of_language (language_of_query q)))
+      | Q_nnrs_imp _ => Ev_out_unsupported ("No debug evaluation support for "++(name_of_language (language_of_query q)))
       | Q_nnrcmr _ => Ev_out_unsupported ("No debug evaluation support for "++(name_of_language (language_of_query q)))
       | Q_cldmr _ => Ev_out_unsupported ("No debug evaluation support for "++(name_of_language (language_of_query q)))
       | Q_dnnrc _ => Ev_out_unsupported ("No debug evaluation support for "++(name_of_language (language_of_query q)))
@@ -301,8 +301,8 @@ Section CompEval.
     Definition eval_nnrs_world (q:nnrs) (world:list data) : option data :=
       eval_nnrs q (mkWorld world).
 
-    Definition eval_nnrc_imp_world (q:nnrc_imp) (world:list data) : option data :=
-      eval_nnrc_imp q (mkWorld world).
+    Definition eval_nnrs_imp_world (q:nnrs_imp) (world:list data) : option data :=
+      eval_nnrs_imp q (mkWorld world).
 
     Definition eval_nnrcmr_world (q:nnrcmr) (world:list data) : option data :=
       eval_nnrcmr q (mkDistWorld world). (* XXX Creates a distributed WORLD collection XXX *)
