coq/Compiler/Driver/CompLang.v
@@ -35,7 +35,7 @@ Require Import NRARuntime.
 Require Import NRAEnvRuntime.
 Require Import NNRCRuntime.
 Require Import NNRSRuntime.
-Require Import NNRCimpRuntime.
+Require Import NNRSimpRuntime.
 Require Import NNRCMRRuntime.
 Require Import CldMRRuntime.
 Require Import DNNRCRuntime.
@@ -70,7 +70,7 @@ Section CompLang.
     | L_nnrc : language
     | L_nnrs_core : language
     | L_nnrs : language
-    | L_nnrc_imp : language
+    | L_nnrs_imp : language
     | L_nnrcmr : language
     | L_cldmr : language
     | L_dnnrc : language
@@ -117,7 +117,7 @@ Section CompLang.
       | "nnrc"%string => L_nnrc
       | "nnrs_core"%string => L_nnrs_core
       | "nnrs"%string => L_nnrs
-      | "nnrc_imp"%string => L_nnrc_imp
+      | "nnrs_imp"%string => L_nnrs_imp
       | "nnrcmr"%string => L_nnrcmr
       | "cldmr"%string => L_cldmr
       | "dnnrc"%string => L_dnnrc
@@ -149,7 +149,7 @@ Section CompLang.
       | L_nnrc => "nnrc"%string
       | L_nnrs_core => "nnrs_core"%string
       | L_nnrs => "nnrs"%string
-      | L_nnrc_imp => "nnrc_imp"%string
+      | L_nnrs_imp => "nnrs_imp"%string
       | L_nnrcmr => "nnrcmr"%string
       | L_cldmr => "cldmr"%string
       | L_dnnrc => "dnnrc"%string
@@ -211,7 +211,7 @@ Section CompLang.
         :: (L_nnrc,CoreEnd,"NNRC", "Named Nested Relational Calculus")
         :: (L_nnrs_core,BackEnd,"cNNRS", "Core Named Nested Relational Calculus imperative")
         :: (L_nnrs,BackEnd,"NNRS", "Named Nested Relational Calculus imperative")
-        :: (L_nnrc_imp,BackEnd,"NNRCimp", "Named Nested Relational Calculus imperative")
+        :: (L_nnrs_imp,BackEnd,"NNRSimp", "Named Nested Relational Calculus imperative")
         :: (L_nnrcmr,DistrEnd,"NNRCMR", "Named Nested Relational Calculus with Map/Reduce")
         :: (L_cldmr,DistrEnd,"CldMR", "Named Nested Relational Calculus with Cloudant Map/Reduce")
         :: (L_dnnrc,DistrEnd,"DNNRC", "Distributed Named Nested Relational Calculus")
@@ -304,7 +304,7 @@ Section CompLang.
     Definition nnrc := nnrc.
     Definition nnrs_core := nnrs_core.
     Definition nnrs := nnrs.
-    Definition nnrc_imp := nnrc_imp.
+    Definition nnrs_imp := nnrs_imp.
     Definition nnrcmr := nnrcmr.
     Definition cldmr := cldmr.
     Definition dnnrc := dnnrc.
@@ -332,7 +332,7 @@ Section CompLang.
     | Q_nnrc : nnrc -> query
     | Q_nnrs_core : nnrs_core -> query
     | Q_nnrs : nnrs -> query
-    | Q_nnrc_imp : nnrc_imp -> query
+    | Q_nnrs_imp : nnrs_imp -> query
     | Q_nnrcmr : nnrcmr -> query
     | Q_cldmr : cldmr -> query
     | Q_dnnrc : dnnrc -> query
@@ -362,7 +362,7 @@ Section CompLang.
       | Case_aux c "Q_nnrc"%string
       | Case_aux c "Q_nnrs_core"%string
       | Case_aux c "Q_nnrs"%string
-      | Case_aux c "Q_nnrc_imp"%string
+      | Case_aux c "Q_nnrs_imp"%string
       | Case_aux c "Q_nnrcmr"%string
       | Case_aux c "Q_cldmr"%string
       | Case_aux c "Q_dnnrc"%string
@@ -392,7 +392,7 @@ Section CompLang.
       | Q_nnrc _ => L_nnrc
       | Q_nnrs_core _ => L_nnrs_core
       | Q_nnrs _ => L_nnrs
-      | Q_nnrc_imp _ => L_nnrc_imp
+      | Q_nnrs_imp _ => L_nnrs_imp
       | Q_nnrcmr _ => L_nnrcmr
       | Q_cldmr _ => L_cldmr
       | Q_dnnrc _ => L_dnnrc
@@ -428,7 +428,7 @@ Section CompLang.
       | L_nnrc => nnrc
       | L_nnrs_core => nnrs_core
       | L_nnrs => nnrs
-      | L_nnrc_imp => nnrc_imp
+      | L_nnrs_imp => nnrs_imp
       | L_nnrcmr => nnrcmr
       | L_cldmr => cldmr
       | L_dnnrc => dnnrc
@@ -462,7 +462,7 @@ Tactic Notation "language_cases" tactic(first) ident(c) :=
   | Case_aux c "L_nnrc"%string
   | Case_aux c "L_nnrs_core"%string
   | Case_aux c "L_nnrs"%string
-  | Case_aux c "L_nnrc_imp"%string
+  | Case_aux c "L_nnrs_imp"%string
   | Case_aux c "L_nnrcmr"%string
   | Case_aux c "L_cldmr"%string
   | Case_aux c "L_dnnrc"%string
