coq/NNRSimp/Lang/NNRSimpEval.v
@@ -14,7 +14,7 @@
  * limitations under the License.
  *)
 
-(** NNRCimp is a variant of the named nested relational calculus
+(** NNRSimp is a variant of the named nested relational calculus
      (NNRC) that is meant to be more imperative in feel.  It is used
      as an intermediate language between NNRC and more imperative /
      statement oriented backends *)
@@ -32,88 +32,88 @@ Require Import EquivDec.
 Require Import Decidable.
 Require Import Utils.
 Require Import CommonRuntime.
-Require Import NNRCimp.
-Require Import NNRCimpVars.
+Require Import NNRSimp.
+Require Import NNRSimpVars.
 
-Section NNRCimpEval.
+Section NNRSimpEval.
 
   Context {fruntime:foreign_runtime}.
 
   Context (h:brand_relation_t).
 
-  Local Open Scope nnrc_imp.
+  Local Open Scope nnrs_imp.
   Local Open Scope string.
 
   (** ** Evaluation Semantics *)
   Section Evaluation.
 
-    (** Evaluation takes a NNRCimp expression and an environment. It
+    (** Evaluation takes a NNRSimp expression and an environment. It
           returns an optional value. When [None] is returned, it
           denotes an error. An error is always propagated. *)
 
-    Fixpoint nnrc_imp_expr_eval
-             (σc:bindings) (σ:pd_bindings) (e:nnrc_imp_expr)
+    Fixpoint nnrs_imp_expr_eval
+             (σc:bindings) (σ:pd_bindings) (e:nnrs_imp_expr)
     : option data
       := match e with
-         | NNRCimpGetConstant v =>
+         | NNRSimpGetConstant v =>
            edot σc v
 
-         | NNRCimpVar v =>
+         | NNRSimpVar v =>
            olift id (lookup equiv_dec σ v)
 
-         | NNRCimpConst d =>
+         | NNRSimpConst d =>
            Some (normalize_data h d)
 
-         | NNRCimpBinop bop e₁ e₂ =>
+         | NNRSimpBinop bop e₁ e₂ =>
            olift2 (fun d₁ d₂ => binary_op_eval h bop d₁ d₂)
-                  (nnrc_imp_expr_eval σc σ e₁)
-                  (nnrc_imp_expr_eval σc σ e₂)
+                  (nnrs_imp_expr_eval σc σ e₁)
+                  (nnrs_imp_expr_eval σc σ e₂)
 
-         | NNRCimpUnop uop e =>
+         | NNRSimpUnop uop e =>
            olift (fun d => unary_op_eval h uop d)
-                 (nnrc_imp_expr_eval σc σ e)
+                 (nnrs_imp_expr_eval σc σ e)
 
-         | NNRCimpGroupBy g sl e =>
-           match nnrc_imp_expr_eval σc σ e with
+         | NNRSimpGroupBy g sl e =>
+           match nnrs_imp_expr_eval σc σ e with
            | Some (dcoll dl) => lift dcoll (group_by_nested_eval_table g sl dl)
            | _ => None
            end
          end.
 
 
-    Fixpoint nnrc_imp_stmt_eval
-             (σc:bindings) (s:nnrc_imp_stmt) 
+    Fixpoint nnrs_imp_stmt_eval
+             (σc:bindings) (s:nnrs_imp_stmt) 
              (σ:pd_bindings) : option (pd_bindings)
       := match s with
-         | NNRCimpSeq s₁ s₂ =>
-           olift (nnrc_imp_stmt_eval σc s₂)
-                 (nnrc_imp_stmt_eval σc s₁ σ)
+         | NNRSimpSeq s₁ s₂ =>
+           olift (nnrs_imp_stmt_eval σc s₂)
+                 (nnrs_imp_stmt_eval σc s₁ σ)
                  
-         | NNRCimpAssign v e =>
-           match nnrc_imp_expr_eval σc σ e, lookup string_dec σ v with
+         | NNRSimpAssign v e =>
+           match nnrs_imp_expr_eval σc σ e, lookup string_dec σ v with
            | Some d, Some _ => Some (update_first string_dec σ v (Some d))
            | _, _ => None
            end
              
-         | NNRCimpLet v eo s₀ =>
+         | NNRSimpLet v eo s₀ =>
            let evals := (fun init =>
-                           match nnrc_imp_stmt_eval σc s₀ ((v,init)::σ) with
+                           match nnrs_imp_stmt_eval σc s₀ ((v,init)::σ) with
                            | Some (_::σ') => Some σ'
                            | _ => None
                            end) in
            match eo with
-           | Some e => olift evals (lift Some (nnrc_imp_expr_eval σc σ e))
+           | Some e => olift evals (lift Some (nnrs_imp_expr_eval σc σ e))
            | None => evals None
            end
              
-         | NNRCimpFor v e s₀ =>
-           match nnrc_imp_expr_eval σc σ e with
+         | NNRSimpFor v e s₀ =>
+           match nnrs_imp_expr_eval σc σ e with
            | Some (dcoll c1) =>
              let fix for_fun (dl:list data) σ₁ :=
                  match dl with
                  | nil => Some σ₁
                  | d::dl' =>
-                   match nnrc_imp_stmt_eval σc s₀ ((v,Some d)::σ₁) with
+                   match nnrs_imp_stmt_eval σc s₀ ((v,Some d)::σ₁) with
                    | Some (_::σ₂) => for_fun dl' σ₂ 
                    | _ => None
                    end
@@ -122,22 +122,22 @@ Section NNRCimpEval.
            | _ => None
            end
 
-         | NNRCimpIf e s₁ s₂ =>
-           match nnrc_imp_expr_eval σc σ e  with
-           | Some (dbool true) => nnrc_imp_stmt_eval σc s₁ σ
-           | Some (dbool false) => nnrc_imp_stmt_eval σc s₂ σ
+         | NNRSimpIf e s₁ s₂ =>
+           match nnrs_imp_expr_eval σc σ e  with
+           | Some (dbool true) => nnrs_imp_stmt_eval σc s₁ σ
+           | Some (dbool false) => nnrs_imp_stmt_eval σc s₂ σ
            | _ => None
            end
 
-         | NNRCimpEither e x₁ s₁ x₂ s₂ =>
-           match nnrc_imp_expr_eval σc σ e with
+         | NNRSimpEither e x₁ s₁ x₂ s₂ =>
+           match nnrs_imp_expr_eval σc σ e with
            | Some (dleft d) =>
-             match nnrc_imp_stmt_eval σc s₁ ((x₁,Some d)::σ) with
+             match nnrs_imp_stmt_eval σc s₁ ((x₁,Some d)::σ) with
              | Some (_::σ₂) => Some σ₂
              | _ => None
              end
            | Some (dright d) =>
-             match nnrc_imp_stmt_eval σc s₂ ((x₂,Some d)::σ) with
+             match nnrs_imp_stmt_eval σc s₂ ((x₂,Some d)::σ) with
              | Some (_::σ₂) => Some σ₂
              | _ => None
              end
@@ -145,24 +145,24 @@ Section NNRCimpEval.
            end
          end.
 
-    Definition nnrc_imp_eval σc (q:nnrc_imp) : option (option data) :=
+    Definition nnrs_imp_eval σc (q:nnrs_imp) : option (option data) :=
       let (s, ret) := q in
-      match nnrc_imp_stmt_eval σc s ((ret, None)::nil) with
+      match nnrs_imp_stmt_eval σc s ((ret, None)::nil) with
       | Some ((_,o)::_) => Some o
       | _ => None
       end.
 
-    Definition nnrc_imp_eval_top σc (q:nnrc_imp) :=
-      olift id (nnrc_imp_eval (rec_sort σc) q).
+    Definition nnrs_imp_eval_top σc (q:nnrs_imp) :=
+      olift id (nnrs_imp_eval (rec_sort σc) q).
 
   End Evaluation.
 
   Section Core.
-    Program Definition nnrc_imp_core_eval σc (q:nnrc_imp_core)
-      := nnrc_imp_eval σc q.
+    Program Definition nnrs_imp_core_eval σc (q:nnrs_imp_core)
+      := nnrs_imp_eval σc q.
 
-    Program Definition nnrc_imp_core_eval_top σc (q:nnrc_imp_core)
-      :=  olift id (nnrc_imp_core_eval (rec_sort σc) q).
+    Program Definition nnrs_imp_core_eval_top σc (q:nnrs_imp_core)
+      :=  olift id (nnrs_imp_core_eval (rec_sort σc) q).
     
   End Core.
 
@@ -188,19 +188,19 @@ Section NNRCimpEval.
              [intros eqq | intros ? eqq]; try rewrite eqq in H; try discriminate)
         ]; subst.
 
-    Lemma nnrc_imp_stmt_eval_env_domain_stack {s σc σ₁ σ₂} :
-      nnrc_imp_stmt_eval σc s σ₁ = Some σ₂ -> domain σ₁ = domain σ₂.
+    Lemma nnrs_imp_stmt_eval_env_domain_stack {s σc σ₁ σ₂} :
+      nnrs_imp_stmt_eval σc s σ₁ = Some σ₂ -> domain σ₁ = domain σ₂.
     Proof.
       revert σ₁ σ₂.
-      nnrc_imp_stmt_cases (induction s) Case; intros σ₁ σ₂ sem; simpl in sem; repeat destr sem.
-      - Case "NNRCimpSeq".
+      nnrs_imp_stmt_cases (induction s) Case; intros σ₁ σ₂ sem; simpl in sem; repeat destr sem.
+      - Case "NNRSimpSeq".
         apply some_olift in sem.
         destruct sem as [σ' ? ?].
         transitivity (domain σ'); eauto.
-      - Case "NNRCimpAssign".
+      - Case "NNRSimpAssign".
         invcs sem.
         rewrite domain_update_first; trivial.
-      - Case "NNRCimpLet".
+      - Case "NNRSimpLet".
         apply some_olift in sem.
         destruct sem as [d eqq1 eqq2 ].
         match_option_in eqq2.
@@ -208,11 +208,11 @@ Section NNRCimpEval.
         invcs eqq2.
         specialize (IHs _ _ eqq).
         simpl in IHs; invcs IHs; trivial.
-      - Case "NNRCimpLet".
+      - Case "NNRSimpLet".
         invcs sem.
         specialize (IHs _ _ eqq).
         simpl in IHs; invcs IHs; trivial.
-      - Case  "NNRCimpFor".
+      - Case  "NNRSimpFor".
         destruct d; try discriminate.
         clear eqq.
         revert σ₁ σ₂ sem.
@@ -222,10 +222,10 @@ Section NNRCimpEval.
         specialize (IHs _ _ eqq).
         simpl in IHs; invcs IHs.
         congruence.
-      - Case "NNRCimpIf".
+      - Case "NNRSimpIf".
         destruct d; try discriminate.
         destruct b; eauto.
-      - Case "NNRCimpEither".
+      - Case "NNRSimpEither".
         destruct d; try discriminate;
           repeat destr sem; invcs sem.
         + specialize (IHs1 _ _ eqq0);
@@ -234,9 +234,9 @@ Section NNRCimpEval.
             simpl in IHs2; invcs IHs2; trivial.
     Qed.
 
-    Lemma nnrc_imp_expr_eval_same σc pd₁ pd₂ s :
-      lookup_equiv_on (nnrc_imp_expr_free_vars s) pd₁ pd₂ ->
-      nnrc_imp_expr_eval σc pd₁ s = nnrc_imp_expr_eval σc pd₂ s.
+    Lemma nnrs_imp_expr_eval_same σc pd₁ pd₂ s :
+      lookup_equiv_on (nnrs_imp_expr_free_vars s) pd₁ pd₂ ->
+      nnrs_imp_expr_eval σc pd₁ s = nnrs_imp_expr_eval σc pd₂ s.
     Proof.
       revert pd₁ pd₂.
       induction s; simpl; intros; eauto 3.
@@ -249,9 +249,9 @@ Section NNRCimpEval.
       - rewrite (IHs _ _ H); trivial.
     Qed.
 
-    Lemma nnrc_imp_expr_eval_group_by_unfold σc σ g sl e :
-      nnrc_imp_expr_eval σc σ (NNRCimpGroupBy g sl e) = 
-      match nnrc_imp_expr_eval σc σ e with
+    Lemma nnrs_imp_expr_eval_group_by_unfold σc σ g sl e :
+      nnrs_imp_expr_eval σc σ (NNRSimpGroupBy g sl e) = 
+      match nnrs_imp_expr_eval σc σ e with
       | Some (dcoll dl) => lift dcoll (group_by_nested_eval_table g sl dl)
       | _ => None
       end.
@@ -259,16 +259,16 @@ Section NNRCimpEval.
       reflexivity.
     Qed.
 
-    Global Instance nnrc_imp_expr_eval_proper 
-      : Proper (eq ==> lookup_equiv ==> eq ==> eq) nnrc_imp_expr_eval.
+    Global Instance nnrs_imp_expr_eval_proper 
+      : Proper (eq ==> lookup_equiv ==> eq ==> eq) nnrs_imp_expr_eval.
     Proof.
       intros ?????????; subst.
-      apply nnrc_imp_expr_eval_same.
+      apply nnrs_imp_expr_eval_same.
       apply lookup_equiv_on_lookup_equiv; trivial.
     Qed.
 
   End props.
 
-End NNRCimpEval.
+End NNRSimpEval.
 
-Arguments nnrc_imp_stmt_eval_env_domain_stack {fruntime h s σc σ₁ σ₂}.
+Arguments nnrs_imp_stmt_eval_env_domain_stack {fruntime h s σc σ₁ σ₂}.
