coq/Compiler/Driver/CompStat.v
@@ -32,7 +32,7 @@ Require Import NRARuntime.
 Require Import NRAEnvRuntime.
 Require Import NNRCRuntime.
 Require Import NNRSRuntime.
-Require Import NNRCimpRuntime.
+Require Import NNRSimpRuntime.
 Require Import NNRCMRRuntime.
 Require Import CldMRRuntime.
 Require Import DNNRCRuntime.
@@ -131,9 +131,9 @@ Section CompStat.
       (("nnrcmr_length", dnat (Z_of_nat (List.length q.(mr_chain))))
          :: nil).
 
-  Definition stat_nnrc_imp (q: nnrc_imp) : data :=
+  Definition stat_nnrs_imp (q: nnrs_imp) : data :=
     drec
-      (("nnrc_imp_size", dnat (Z_of_nat (nnrc_imp_size q)))
+      (("nnrs_imp_size", dnat (Z_of_nat (nnrs_imp_size q)))
          :: nil).
 
   Definition stat_nnrs_core (q: nnrs_core) : data :=
@@ -276,9 +276,9 @@ Section CompStat.
          :: ("nnrcmr_optim_time", dstring t)
          :: nil).
 
-  Definition stat_tree_nnrc_imp (q: nnrc_imp) : data :=
+  Definition stat_tree_nnrs_imp (q: nnrs_imp) : data :=
     drec
-      (("nnrc_imp", stat_nnrc_imp q)
+      (("nnrs_imp", stat_nnrs_imp q)
          :: nil).
 
   Definition stat_tree_nnrs_core (q: nnrs_core) : data :=
@@ -463,7 +463,7 @@ Section CompStat.
         | Q_nnrc q => stat_nnrc q
         | Q_nnrs_core q => stat_nnrs_core q
         | Q_nnrs q => stat_nnrs q
-        | Q_nnrc_imp q => stat_nnrc_imp q
+        | Q_nnrs_imp q => stat_nnrs_imp q
         | Q_nnrcmr q => stat_nnrcmr q
         | Q_cldmr q => stat_cldmr q
         | Q_dnnrc q => stat_dnnrc q
@@ -497,7 +497,7 @@ Section CompStat.
         | Q_nnrc q => stat_tree_nnrc q
         | Q_nnrs_core q => stat_tree_nnrs_core q
         | Q_nnrs q => stat_tree_nnrs q
-        | Q_nnrc_imp q => stat_tree_nnrc_imp q
+        | Q_nnrs_imp q => stat_tree_nnrs_imp q
         | Q_nnrcmr q => stat_tree_nnrcmr q
         | Q_cldmr q => stat_tree_cldmr q
         | Q_dnnrc q => stat_tree_dnnrc q
