coq/NNRSimp/Lang/NNRSimp.v
@@ -1,0 +1,267 @@
+(*
+ * Copyright 2015-2016 IBM Corporation
+ *
+ * Licensed under the Apache License, Version 2.0 (the "License");
+ * you may not use this file except in compliance with the License.
+ * You may obtain a copy of the License at
+ *
+ * http://www.apache.org/licenses/LICENSE-2.0
+ *
+ * Unless required by applicable law or agreed to in writing, software
+ * distributed under the License is distributed on an "AS IS" BASIS,
+ * WITHOUT WARRANTIES OR CONDITIONS OF ANY KIND, either express or implied.
+ * See the License for the specific language governing permissions and
+ * limitations under the License.
+ *)
+
+(** NNRSimp is a variant of the named nested relational calculus
+     (NNRC) that is meant to be more imperative in feel.  It is used
+     as an intermediate language between NNRC and more imperative /
+     statement oriented backends *)
+
+Require Import String.
+Require Import List.
+Require Import Arith.
+Require Import EquivDec.
+Require Import Morphisms.
+Require Import Arith.
+Require Import Max.
+Require Import Bool.
+Require Import Peano_dec.
+Require Import EquivDec.
+Require Import Decidable.
+Require Import Utils.
+Require Import CommonRuntime.
+  
+Section NNRSimp.
+
+  Section Syntax.
+
+    Context {fruntime:foreign_runtime}.
+
+    Inductive nnrs_imp_expr :=
+    | NNRSimpGetConstant : var -> nnrs_imp_expr                                   (**r global variable lookup ([$$v]) *)
+    | NNRSimpVar : var -> nnrs_imp_expr                                           (**r local variable lookup ([$v])*)
+    | NNRSimpConst : data -> nnrs_imp_expr                                        (**r constant data ([d]) *)
+    | NNRSimpBinop : binary_op -> nnrs_imp_expr -> nnrs_imp_expr -> nnrs_imp_expr (**r binary operator ([e₁ ⊠ e₂]) *)
+    | NNRSimpUnop : unary_op -> nnrs_imp_expr -> nnrs_imp_expr                    (**r unary operator ([⊞ e]) *)
+    | NNRSimpGroupBy : string -> list string -> nnrs_imp_expr -> nnrs_imp_expr    (**r group by expression ([e groupby g fields]) -- only in full NNRC *)
+    .
+
+    Inductive nnrs_imp_stmt :=
+    | NNRSimpSeq : nnrs_imp_stmt -> nnrs_imp_stmt -> nnrs_imp_stmt                    (**r sequence ([s₁; s₂]]) *)
+    | NNRSimpAssign : var -> nnrs_imp_expr -> nnrs_imp_stmt                           (**r variable assignent ([$v := e]) *)
+    | NNRSimpLet : var -> option nnrs_imp_expr -> nnrs_imp_stmt -> nnrs_imp_stmt (**r variable declaration ([var $v := e₁?; s₂]) *)
+    | NNRSimpFor : var -> nnrs_imp_expr -> nnrs_imp_stmt -> nnrs_imp_stmt             (**r for loop ([for ($v in e₁) { s₂ }]) *)
+    | NNRSimpIf : nnrs_imp_expr -> nnrs_imp_stmt -> nnrs_imp_stmt -> nnrs_imp_stmt    (**r conditional ([if e₁ { s₂ } else { s₃ }]) *)
+    | NNRSimpEither : nnrs_imp_expr                                                   (**r case expression ([either e case left $v₁ { s₁ } case right $v₂ { s₂ }]) *)
+                      -> var -> nnrs_imp_stmt
+                      -> var -> nnrs_imp_stmt -> nnrs_imp_stmt
+    .
+
+    (** [nnrs_imp] is composed of the statement evaluating the query
+        and the variable containing the result of the evaluation *)
+    Definition nnrs_imp : Set := (nnrs_imp_stmt * var).
+
+    (* Note: `Let x = e in s' should be equivalent to `for (x<-{e}) in s' *)
+    (* which should be the same as `either (dleft e) (x->s) (_->_) ' *)
+    
+  End Syntax.
+
+  Section dec.
+    Context {fruntime:foreign_runtime}.
+
+    Global Instance nnrs_imp_expr_eqdec : EqDec nnrs_imp_expr eq.
+    Proof.
+      change (forall x y : nnrs_imp_expr,  {x = y} + {x <> y}).
+      decide equality;
+        try solve [apply binary_op_eqdec | apply unary_op_eqdec
+                   | apply data_eqdec | apply string_eqdec].
+      - decide equality; apply string_dec.
+    Defined.
+
+    Global Instance nnrs_imp_stmt_eqdec : EqDec nnrs_imp_stmt eq.
+    Proof.
+      change (forall x y : nnrs_imp_stmt,  {x = y} + {x <> y}).
+      decide equality;
+        try solve [apply nnrs_imp_expr_eqdec | apply string_eqdec | apply option_eqdec].
+    Defined.
+
+    Global Instance nnrs_imp_eqdec : EqDec nnrs_imp eq.
+    Proof.
+      intros [s1 r1] [s2 r2].
+      destruct (r1 == r2).
+      - destruct (s1 == s2).
+        + left; congruence.
+        + right; congruence.
+      - right; congruence.
+    Defined.
+  End dec.
+
+  Section Core.
+
+    Context {fruntime:foreign_runtime}.
+
+    Fixpoint nnrs_imp_exprIsCore (e:nnrs_imp_expr) : Prop :=
+      match e with
+      | NNRSimpGetConstant _ => True
+      | NNRSimpVar _ => True
+      | NNRSimpConst _ => True
+      | NNRSimpBinop _ e1 e2 => nnrs_imp_exprIsCore e1 /\ nnrs_imp_exprIsCore e2
+      | NNRSimpUnop _ e1 => nnrs_imp_exprIsCore e1
+      | NNRSimpGroupBy _ _ _ => False
+      end.
+    
+    Fixpoint nnrs_imp_stmtIsCore (s:nnrs_imp_stmt) : Prop :=
+      match s with
+      | NNRSimpSeq s1 s2 =>
+        nnrs_imp_stmtIsCore s1 /\ nnrs_imp_stmtIsCore s2
+      | NNRSimpLet _ (Some e) s1 =>
+        nnrs_imp_exprIsCore e /\ nnrs_imp_stmtIsCore s1
+      | NNRSimpLet _ None s1 =>
+        nnrs_imp_stmtIsCore s1
+      | NNRSimpAssign _ e =>
+        nnrs_imp_exprIsCore e
+      | NNRSimpFor _ e s1 =>
+        nnrs_imp_exprIsCore e /\ nnrs_imp_stmtIsCore s1
+      | NNRSimpIf e s1 s2 =>
+        nnrs_imp_exprIsCore e /\ nnrs_imp_stmtIsCore s1 /\ nnrs_imp_stmtIsCore s2
+      | NNRSimpEither e _ s1 _ s2 =>
+        nnrs_imp_exprIsCore e /\ nnrs_imp_stmtIsCore s1 /\ nnrs_imp_stmtIsCore s2
+      end .
+
+    Definition nnrs_impIsCore (sr:nnrs_imp) := nnrs_imp_stmtIsCore (fst sr).
+
+    Definition nnrs_imp_core : Set := {sr:nnrs_imp | nnrs_impIsCore sr}.
+
+    Definition nnrs_imp_core_to_nnrs_imp (sr:nnrs_imp_core) : nnrs_imp :=
+      proj1_sig sr.
+
+    Section ext.
+
+      Lemma nnrs_imp_exprIsCore_ext (e:nnrs_imp_expr) (pf1 pf2:nnrs_imp_exprIsCore e) : pf1 = pf2.
+      Proof.
+        induction e; simpl in *;
+          try (destruct pf1; destruct pf2; trivial);
+          try f_equal; auto.
+      Qed.
+
+      Lemma nnrs_imp_stmtIsCore_ext (s:nnrs_imp_stmt) (pf1 pf2:nnrs_imp_stmtIsCore s) : pf1 = pf2.
+      Proof.
+        induction s; simpl in *;
+          try (destruct o);
+          try (destruct pf1; destruct pf2; trivial);
+          try (destruct a; destruct a0);
+          try f_equal; eauto;
+            try eapply nnrs_imp_exprIsCore_ext; eauto
+            ; try f_equal; eauto.
+      Qed.
+
+      Lemma nnrs_impIsCore_ext (e:nnrs_imp) (pf1 pf2:nnrs_impIsCore e) : pf1 = pf2.
+      Proof.
+        apply nnrs_imp_stmtIsCore_ext.
+      Qed.
+
+      Lemma nnrs_imp_core_ext e (pf1 pf2:nnrs_impIsCore e) :
+        exist _ e pf1 = exist _ e pf2.
+      Proof.
+        f_equal; apply nnrs_impIsCore_ext.
+      Qed.
+
+      Lemma nnrs_imp_core_fequal (e1 e2:nnrs_imp_core) :
+        proj1_sig e1 = proj1_sig e2 -> e1 = e2.
+      Proof.
+        destruct e1; destruct e2; simpl; intros eqq.
+        destruct eqq.
+        apply nnrs_imp_core_ext.
+      Qed.
+
+    End ext.
+    
+    Section dec.
+
+      Lemma nnrs_imp_exprIsCore_dec (e:nnrs_imp_expr) :
+        {nnrs_imp_exprIsCore e} + {~ nnrs_imp_exprIsCore e}.
+      Proof.
+        induction e; simpl; try eauto 3.
+        destruct IHe1.
+        - destruct IHe2; [left|right]; intuition.
+        - right; intuition.
+      Defined.
+
+      Lemma nnrs_imp_stmtIsCore_dec (s:nnrs_imp_stmt) :
+        {nnrs_imp_stmtIsCore s} + {~ nnrs_imp_stmtIsCore s}.
+      Proof.
+        induction s; simpl.
+        - destruct IHs1.
+          + destruct IHs2; [left|right]; intuition.
+          + right; intuition.
+        - apply (nnrs_imp_exprIsCore_dec n).
+        - destruct o.
+          + destruct (nnrs_imp_exprIsCore_dec n).
+            * destruct IHs; [left|right]; intuition.
+            * right; intuition.
+          + apply IHs.
+        - destruct (nnrs_imp_exprIsCore_dec n).
+          + destruct IHs; [left|right]; intuition.
+          + right; intuition.
+        - destruct (nnrs_imp_exprIsCore_dec n).
+          + destruct IHs1.
+            * destruct IHs2; [left|right]; intuition.
+            * right; intuition.
+          + right; intuition.
+        - destruct (nnrs_imp_exprIsCore_dec n).
+          + destruct IHs1.
+            * destruct IHs2; [left|right]; intuition.
+            * right; intuition.
+          + right; intuition.
+      Defined.
+
+      Lemma nnrs_impIsCore_dec (sr:nnrs_imp) :
+        {nnrs_impIsCore sr} + {~ nnrs_impIsCore sr}.
+      Proof.
+        apply nnrs_imp_stmtIsCore_dec.
+      Defined.
+
+      Global Instance nnrs_imp_core_eqdec : EqDec nnrs_imp_core eq.
+      Proof.
+        intros x y.
+        destruct x as [x xpf]; destruct y as [y ypf].
+        destruct (x == y).
+        - left. apply nnrs_imp_core_fequal; simpl; trivial.
+        - right. inversion 1; congruence.
+      Defined.
+
+    End dec.
+
+End Core.
+
+Section Env.
+  Context {fruntime:foreign_runtime}.
+
+  (* bindings that may or may not be initialized (defined) *)
+  Definition pd_bindings := list (string*option data).
+
+End Env.
+
+End NNRSimp.
+
+Tactic Notation "nnrs_imp_expr_cases" tactic(first) ident(c) :=
+  first;
+  [ Case_aux c "NNRSimpGetConstant"%string
+  | Case_aux c "NNRSimpVar"%string
+  | Case_aux c "NNRSimpConst"%string
+  | Case_aux c "NNRSimpBinop"%string
+  | Case_aux c "NNRSimpUnop"%string
+  | Case_aux c "NNRSimpGroupBy"%string].
+
+Tactic Notation "nnrs_imp_stmt_cases" tactic(first) ident(c) :=
+  first;
+  [ Case_aux c "NNRSimpSeq"%string
+  | Case_aux c "NNRSimpAssign"%string
+  | Case_aux c "NNRSimpLet"%string
+  | Case_aux c "NNRSimpFor"%string
+  | Case_aux c "NNRSimpIf"%string
+  | Case_aux c "NNRSimpEither"%string].
+
+Delimit Scope nnrs_imp with nnrs_imp_scope.
