coq/NNRSimp/Lang/NNRSimpSem.v
@@ -1,0 +1,242 @@
+(*
+ * Copyright 2015-2016 IBM Corporation
+ *
+ * Licensed under the Apache License, Version 2.0 (the "License");
+ * you may not use this file except in compliance with the License.
+ * You may obtain a copy of the License at
+ *
+ * http://www.apache.org/licenses/LICENSE-2.0
+ *
+ * Unless required by applicable law or agreed to in writing, software
+ * distributed under the License is distributed on an "AS IS" BASIS,
+ * WITHOUT WARRANTIES OR CONDITIONS OF ANY KIND, either express or implied.
+ * See the License for the specific language governing permissions and
+ * limitations under the License.
+ *)
+
+(** NNRSimp is a variant of the named nested relational calculus
+     (NNRC) that is meant to be more imperative in feel.  It is used
+     as an intermediate language between NNRC and more imperative /
+     statement oriented backends *)
+
+Require Import String.
+Require Import List.
+Require Import Arith.
+Require Import EquivDec.
+Require Import Morphisms.
+Require Import Arith.
+Require Import Max.
+Require Import Bool.
+Require Import Peano_dec.
+Require Import EquivDec.
+Require Import Decidable.
+Require Import Utils.
+Require Import CommonRuntime.
+Require Import NNRSimp.
+
+Section NNRSimpSem.
+
+  Context {fruntime:foreign_runtime}.
+
+  Context (h:brand_relation_t).
+
+  Local Open Scope nnrs_imp.
+  Local Open Scope string.
+
+  Section Denotation.
+    Context (σc:list (string*data)).
+
+    Reserved Notation  "[ σ ⊢ e ⇓ d ]".
+
+    Inductive nnrs_imp_expr_sem : pd_bindings -> nnrs_imp_expr -> data -> Prop :=
+    | sem_NNRSimpGetConstant : forall v σ d,
+        edot σc v = Some d ->                 (**r   [Γc(v) = d] *)
+        [ σ ⊢ NNRSimpGetConstant v ⇓ d ]
+
+    | sem_NNRSimpVar : forall v σ d,
+        lookup equiv_dec σ v = Some (Some d) ->              (**r   [Γ(v) = d] *)
+        [ σ ⊢ NNRSimpVar v ⇓ d ]
+
+    | sem_NNRSimpConst : forall d₁ σ d₂,
+        normalize_data h d₁ = d₂ ->                     (**r   [norm(d₁) = d₂] *)
+        [ σ ⊢ NNRSimpConst d₁ ⇓ d₂ ]
+
+    | sem_NNRSimpBinop : forall bop e₁ e₂ σ d₁ d₂ d,
+        [ σ ⊢ e₁ ⇓ d₁ ] ->
+        [ σ ⊢ e₂ ⇓ d₂ ] ->
+        binary_op_eval h bop d₁ d₂ = Some d ->
+        [ σ ⊢ NNRSimpBinop bop e₁ e₂ ⇓ d ]
+
+    | sem_NNRSimpUnop : forall uop e σ d₁ d,
+        [ σ ⊢ e ⇓ d₁ ] ->
+        unary_op_eval h uop d₁ = Some d ->
+        [ σ ⊢ NNRSimpUnop uop e ⇓ d ]
+
+    | sem_NNRSimpGroupBy : forall g sl e σ d₁ d₂ ,
+        [ σ ⊢ e ⇓ (dcoll d₁) ] ->
+        group_by_nested_eval_table g sl d₁ = Some d₂ ->
+        [ σ ⊢ NNRSimpGroupBy g sl e ⇓ (dcoll d₂) ]
+
+    where
+    "[ σ ⊢ e ⇓ d ]" := (nnrs_imp_expr_sem σ e d) : nnrs_imp
+    .
+
+    Reserved Notation  "[ s₁ , σ₁ ⇓ σ₂  ]".
+    Reserved Notation "[ s , σ₁ ⇓[ v <- dl ] σ₂ ]".
+    
+    Inductive nnrs_imp_stmt_sem : nnrs_imp_stmt -> pd_bindings -> pd_bindings -> Prop :=
+    | sem_NNRSimpSeq s₁ s₂ σ₁ σ₂ σ₃  :
+        [ s₁, σ₁ ⇓ σ₂ ] ->
+        [ s₂, σ₂ ⇓ σ₃  ] ->
+        [ NNRSimpSeq s₁ s₂, σ₁ ⇓ σ₃ ]
+
+    | sem_NNRSimpAssign v e σ d :
+        In v (domain σ) ->
+        [ σ ⊢ e ⇓ d ] ->
+        [ NNRSimpAssign v e, σ ⇓ update_first string_dec σ v (Some d)]
+
+    | sem_NNRSimpLetNone v s σ₁ σ₂ dd :
+        [ s, (v,None)::σ₁ ⇓ (v,dd)::σ₂ ] ->
+        [ NNRSimpLet v None s, σ₁ ⇓ σ₂  ]
+
+    | sem_NNRSimpLetSome v e s σ₁ σ₂ d dd :
+        [ σ₁ ⊢ e ⇓ d ] ->
+        [ s, (v,Some d)::σ₁ ⇓ (v,dd)::σ₂ ] ->
+        [ NNRSimpLet v (Some e) s, σ₁  ⇓ σ₂ ]
+
+    | sem_NNRSimpFor v e s σ₁ σ₂ dl :
+        [ σ₁ ⊢ e ⇓ (dcoll dl) ] ->
+        [ s, σ₁ ⇓[v<-dl] σ₂ ] ->
+        [ NNRSimpFor v e s, σ₁ ⇓ σ₂ ]
+
+    | sem_NNRSimpIfTrue e s₁ s₂ σ₁ σ₂ :
+        [ σ₁ ⊢ e ⇓ (dbool true) ] ->
+        [ s₁, σ₁ ⇓ σ₂ ] ->
+        [ NNRSimpIf e s₁ s₂, σ₁ ⇓ σ₂ ]
+
+    | sem_NNRSimpIfFalse e s₁ s₂ σ₁ σ₂ :
+        [ σ₁ ⊢ e ⇓ (dbool false) ] ->
+        [ s₂, σ₁ ⇓ σ₂ ] ->
+        [ NNRSimpIf e s₁ s₂, σ₁ ⇓ σ₂ ]
+
+    | sem_NNRSimpEitherLeft e x₁ s₁ x₂ s₂ σ₁ σ₂ d dd :
+        [ σ₁ ⊢ e ⇓ (dleft d) ] ->
+        [ s₁, (x₁,Some d)::σ₁ ⇓ (x₁,dd)::σ₂ ] ->
+        [ NNRSimpEither e x₁ s₁ x₂ s₂, σ₁ ⇓ σ₂]
+
+    | sem_NNRSimpEitherRight e x₁ s₁ x₂ s₂ σ₁ σ₂ d dd :
+        [ σ₁ ⊢ e ⇓ (dright d) ] ->
+        [ s₂, (x₂,Some d)::σ₁ ⇓ (x₂,dd)::σ₂ ] ->
+        [ NNRSimpEither e x₁ s₁ x₂ s₂, σ₁ ⇓ σ₂ ]
+
+    with nnrs_imp_stmt_sem_iter: var -> list data -> nnrs_imp_stmt -> pd_bindings -> pd_bindings ->  Prop :=
+         | sem_NNRSimpIter_nil v s σ :
+             [ s, σ ⇓[v<-nil] σ ]
+         | sem_NNRSimpIter_cons v s σ₁ σ₂ σ₃ d dl dd:
+             [ s, (v,Some d)::σ₁ ⇓ (v,dd)::σ₂] ->
+             [ s, σ₂ ⇓[v<-dl] σ₃ ] ->
+             [ s, σ₁ ⇓[v<-d::dl] σ₃ ]
+    where
+    "[ s , σ₁  ⇓ σ₂ ]" := (nnrs_imp_stmt_sem s σ₁ σ₂) : nnrs_imp
+                                                         and "[ s , σ₁ ⇓[ v <- dl ] σ₂  ]" := (nnrs_imp_stmt_sem_iter v dl s σ₁ σ₂ ) : nnrs_imp.
+
+    Notation "[ s , σ₁ ⇓ σ₂ ]" := (nnrs_imp_stmt_sem s σ₁ σ₂ ) : nnrs_imp.
+    Notation "[ s , σ₁ ⇓[ v <- dl ] σ₂  ]" := (nnrs_imp_stmt_sem_iter v dl s σ₁ σ₂) : nnrs_imp.
+
+  End Denotation.
+
+  Reserved Notation "[ σc ⊢ q ⇓ d  ]".
+
+  Notation "[ σc ; σ ⊢ e ⇓ d ]" := (nnrs_imp_expr_sem σc σ e d) : nnrs_imp.
+  Notation "[ σc ⊢ s , σ₁ ⇓ σ₂ ]" := (nnrs_imp_stmt_sem σc s σ₁ σ₂ ) : nnrs_imp.
+  Notation "[ σc ⊢ s , σ₁ ⇓[ v <- dl ] σ₂ ]" := (nnrs_imp_stmt_sem_iter σc v dl s σ₁ σ₂) : nnrs_imp.
+
+  Inductive nnrs_imp_sem : bindings -> nnrs_imp -> option data -> Prop
+    :=
+    | sem_NNRSimp (σc:bindings) (q: nnrs_imp) o :
+        [ σc ⊢ (fst q), ((snd q),None)::nil ⇓ ((snd q), o)::nil ] ->
+        [ σc ⊢ q ⇓ o  ]
+  where
+  "[ σc ⊢ q ⇓ o  ]" := (nnrs_imp_sem σc q o ) : nnrs_imp.
+
+  Definition nnrs_imp_sem_top (σc:bindings) (q:nnrs_imp) (d:data) : Prop
+    := [ (rec_sort σc) ⊢ q ⇓ Some d  ].
+
+  Notation "[ σc ⊢ q ⇓ d  ]" := (nnrs_imp_sem σc q d ) : nnrs_imp.
+
+  Section Core.
+    Program Definition nnrs_imp_core_sem σc (q:nnrs_imp_core) (d:option data) : Prop
+      := nnrs_imp_sem σc q d.
+
+    Notation "[ σc ⊢ q ⇓ᶜ d  ]" := (nnrs_imp_core_sem σc q d ) : nnrs_imp.
+
+    Definition nnrs_imp_core_sem_top (σc:bindings) (q:nnrs_imp_core) (d:data) : Prop
+      := [ (rec_sort σc) ⊢ q ⇓ᶜ Some d  ].
+
+  End Core.
+
+  Section props.
+
+    Context (σc:list (string*data)).
+    
+    Lemma nnrs_imp_stmt_sem_env_stack {s σ₁ σ₂ }:
+      [ σc ⊢ s, σ₁ ⇓ σ₂  ] -> domain σ₁ = domain σ₂.
+    Proof.
+      revert σ₁ σ₂.
+      nnrs_imp_stmt_cases (induction s) Case; intros σ₁ σ₂ sem; invcs sem.
+      - Case "NNRSimpSeq".
+        transitivity (domain σ₂0); eauto.
+      - Case "NNRSimpAssign".
+        rewrite domain_update_first; trivial.
+      - Case "NNRSimpLet".
+        specialize (IHs _ _ H4).
+        simpl in IHs; invcs IHs.
+        trivial.
+      - Case "NNRSimpLet".
+        specialize (IHs _ _ H5).
+        simpl in IHs; invcs IHs.
+        trivial.
+      - Case  "NNRSimpFor".
+        clear H4.
+        revert σ₁ σ₂ H5.
+        induction dl; intros σ₁ σ₂ sem; invcs sem; trivial.
+        specialize (IHdl  _ _ H6).
+        specialize (IHs _ _ H2).
+        simpl in IHs; invcs IHs.
+        congruence.
+      - Case "NNRSimpIf".
+        eauto.
+      - Case "NNRSimpIf".
+        eauto.
+      - Case "NNRSimpEither".
+        specialize (IHs1 _ _ H7).
+        simpl in IHs1; invcs IHs1; trivial.
+      - Case "NNRSimpEither".
+        specialize (IHs2 _ _ H7).
+        simpl in IHs2; invcs IHs2; trivial.
+    Qed.
+
+    Lemma nnrs_imp_stmt_sem_env_cons_same
+          {s v₁ od₁ σ₁ v₂ od₂ σ₂ } :
+      [ σc ⊢ s, (v₁, od₁) :: σ₁ ⇓ (v₂, od₂) :: σ₂] ->
+      [ σc ⊢ s, (v₁, od₁) :: σ₁ ⇓ (v₁, od₂) :: σ₂ ].
+    Proof.
+      intros sem.
+      generalize (nnrs_imp_stmt_sem_env_stack sem).
+      simpl; intros eqq; invcs eqq.
+      trivial.
+    Qed.
+
+  End props.
+
+End NNRSimpSem.
+
+Notation "[ h , σc ; σ ⊢ e ⇓ d ]" := (nnrs_imp_expr_sem h σc σ e d) : nnrs_imp.
+Notation "[ h , σc ⊢ s , σ₁ ⇓ σ₂ ]" := (nnrs_imp_stmt_sem h σc s σ₁ σ₂ ) : nnrs_imp.
+Notation "[ h , σc ⊢ s , σ₁ ⇓[ v <- dl ] σ₂ ]" := (nnrs_imp_stmt_sem_iter h σc v dl s σ₁ σ₂) : nnrs_imp.
+Notation "[ h , σc ⊢ q ⇓ d  ]" := (nnrs_imp_sem h σc q d ) : nnrs_imp.
+
+Notation "[ h , σc ⊢ q ⇓ᶜ d  ]" := (nnrs_imp_core_sem h σc q d ) : nnrs_imp.
+
+Arguments nnrs_imp_stmt_sem_env_stack {fruntime h σc s σ₁ σ₂}.
+Arguments nnrs_imp_stmt_sem_env_cons_same {fruntime h σc s v₁ od₁ σ₁ v₂ od₂ σ₂}.
