coq/NNRSimp/Lang/NNRSimpSemEval.v
@@ -14,7 +14,7 @@
  * limitations under the License.
  *)
 
-(** NNRCimp is a variant of the named nested relational calculus
+(** NNRSimp is a variant of the named nested relational calculus
      (NNRC) that is meant to be more imperative in feel.  It is used
      as an intermediate language between NNRC and more imperative /
      statement oriented backends *)
@@ -32,54 +32,54 @@ Require Import EquivDec.
 Require Import Decidable.
 Require Import Utils.
 Require Import CommonRuntime.
-Require Import NNRCimp.
-Require Import NNRCimpSem.
-Require Import NNRCimpEval.
+Require Import NNRSimp.
+Require Import NNRSimpSem.
+Require Import NNRSimpEval.
 
-Section NNRCimpSemEval.
+Section NNRSimpSemEval.
 
   Context {fruntime:foreign_runtime}.
 
   Context (h:brand_relation_t).
 
-  Local Open Scope nnrc_imp.
+  Local Open Scope nnrs_imp.
   Local Open Scope string.
 
-  Lemma nnrc_imp_expr_sem_eval σc σ e d :
-    [ h , σc ; σ ⊢ e ⇓ d ] <-> nnrc_imp_expr_eval h σc σ e = Some d.
+  Lemma nnrs_imp_expr_sem_eval σc σ e d :
+    [ h , σc ; σ ⊢ e ⇓ d ] <-> nnrs_imp_expr_eval h σc σ e = Some d.
   Proof.
     split; revert σ d.
     - {
-        nnrc_imp_expr_cases (induction e) Case; intros σ d₀ sem; invcs sem; simpl; trivial.
-        - Case "NNRCimpVar".
+        nnrs_imp_expr_cases (induction e) Case; intros σ d₀ sem; invcs sem; simpl; trivial.
+        - Case "NNRSimpVar".
           rewrite H1; simpl; reflexivity.
-        - Case "NNRCimpBinop".
+        - Case "NNRSimpBinop".
           erewrite IHe1 by eauto.
           erewrite IHe2 by eauto.
           simpl; trivial.
-        - Case "NNRCimpUnop".
+        - Case "NNRSimpUnop".
           erewrite IHe by eauto.
           simpl; trivial.
-        - Case "NNRCimpGroupBy".
+        - Case "NNRSimpGroupBy".
           erewrite IHe by eauto.
           simpl; rewrite H5; simpl; trivial.
       }
     - {
-        Hint Constructors nnrc_imp_expr_sem.
-        nnrc_imp_expr_cases (induction e) Case; intros σ d₀ sem; invcs sem; simpl; trivial; eauto 3.
-        - Case "NNRCimpVar".
+        Hint Constructors nnrs_imp_expr_sem.
+        nnrs_imp_expr_cases (induction e) Case; intros σ d₀ sem; invcs sem; simpl; trivial; eauto 3.
+        - Case "NNRSimpVar".
           apply some_olift in H0.
           destruct H0 as [??]; unfold id in *; subst.
           eauto.
-        - Case "NNRCimpBinop".
+        - Case "NNRSimpBinop".
           apply some_olift2 in H0.
           destruct H0 as [?[?? [??]]].
           eauto.
-        - Case "NNRCimpUnop".
+        - Case "NNRSimpUnop".
           apply some_olift in H0.
           destruct H0 as [??]; unfold id in *; subst.
           eauto.
-        - Case "NNRCimpGroupBy".
+        - Case "NNRSimpGroupBy".
           match_case_in H0;
             [intros ? eqq | intros eqq]; rewrite eqq in H0;
               try discriminate.
@@ -111,63 +111,63 @@ Section NNRCimpSemEval.
            [intros eqq | intros ? eqq]; try rewrite eqq in H; try discriminate)
       ]; subst.
 
-  Lemma nnrc_imp_stmt_sem_eval σc s σ₁ σ₂ :
-    [ h , σc ⊢ s, σ₁ ⇓ σ₂ ] <-> nnrc_imp_stmt_eval h σc s σ₁ = Some σ₂.
+  Lemma nnrs_imp_stmt_sem_eval σc s σ₁ σ₂ :
+    [ h , σc ⊢ s, σ₁ ⇓ σ₂ ] <-> nnrs_imp_stmt_eval h σc s σ₁ = Some σ₂.
   Proof.
     split; revert σ₁ σ₂.
     - {
-        nnrc_imp_stmt_cases (induction s) Case; intros σ₁ σ₂ sem; invcs sem; simpl; trivial.
-        - Case "NNRCimpSeq".
+        nnrs_imp_stmt_cases (induction s) Case; intros σ₁ σ₂ sem; invcs sem; simpl; trivial.
+        - Case "NNRSimpSeq".
           erewrite IHs1 by eauto.
           eauto.
-        - Case "NNRCimpAssign".
-          rewrite nnrc_imp_expr_sem_eval in H4; rewrite H4.
+        - Case "NNRSimpAssign".
+          rewrite nnrs_imp_expr_sem_eval in H4; rewrite H4.
           apply in_dom_lookup with (dec := string_dec) in H1.
           destruct H1 as [? eqq1]; rewrite eqq1; trivial.
-        - Case "NNRCimpLet".
+        - Case "NNRSimpLet".
           erewrite IHs by eauto.
           simpl; trivial.
-        - Case "NNRCimpLet".
-          apply nnrc_imp_expr_sem_eval in H4; rewrite H4; simpl.
+        - Case "NNRSimpLet".
+          apply nnrs_imp_expr_sem_eval in H4; rewrite H4; simpl.
           erewrite IHs by eauto.
           simpl; trivial.
-        - Case "NNRCimpFor".
-          rewrite nnrc_imp_expr_sem_eval in H4; rewrite H4; clear H4.
+        - Case "NNRSimpFor".
+          rewrite nnrs_imp_expr_sem_eval in H4; rewrite H4; clear H4.
           revert σ₁ σ₂ H5.
           induction dl; intros σ₁ σ₂ seval; invcs seval; trivial.
           erewrite IHs by eauto; simpl.
           eauto.
-        - Case "NNRCimpIf".
-          rewrite nnrc_imp_expr_sem_eval in H4; rewrite H4.
+        - Case "NNRSimpIf".
+          rewrite nnrs_imp_expr_sem_eval in H4; rewrite H4.
           eauto.
-        - Case "NNRCimpIf".
-          rewrite nnrc_imp_expr_sem_eval in H4; rewrite H4.
+        - Case "NNRSimpIf".
+          rewrite nnrs_imp_expr_sem_eval in H4; rewrite H4.
           eauto.
-        - Case "NNRCimpEither".
-          rewrite nnrc_imp_expr_sem_eval in H6; rewrite H6.
+        - Case "NNRSimpEither".
+          rewrite nnrs_imp_expr_sem_eval in H6; rewrite H6.
           erewrite IHs1 by eauto.
           simpl; trivial.
-        - Case "NNRCimpEither".
-          rewrite nnrc_imp_expr_sem_eval in H6; rewrite H6.
+        - Case "NNRSimpEither".
+          rewrite nnrs_imp_expr_sem_eval in H6; rewrite H6.
           erewrite IHs2 by eauto.
           simpl; trivial.
       }
     - {
-        Hint Constructors nnrc_imp_stmt_sem.
-        Hint Constructors nnrc_imp_stmt_sem_iter.
-        Hint Resolve nnrc_imp_stmt_sem_env_cons_same.
+        Hint Constructors nnrs_imp_stmt_sem.
+        Hint Constructors nnrs_imp_stmt_sem_iter.
+        Hint Resolve nnrs_imp_stmt_sem_env_cons_same.
 
-        nnrc_imp_stmt_cases (induction s) Case; simpl; intros σ₁ σ₂ sem; repeat destr sem.
-        - Case "NNRCimpSeq".
+        nnrs_imp_stmt_cases (induction s) Case; simpl; intros σ₁ σ₂ sem; repeat destr sem.
+        - Case "NNRSimpSeq".
           apply some_olift in sem.
           destruct sem as [???].
           eauto.
-        - Case "NNRCimpAssign".
+        - Case "NNRSimpAssign".
           invcs sem.
-          apply nnrc_imp_expr_sem_eval in eqq.
+          apply nnrs_imp_expr_sem_eval in eqq.
           apply lookup_in_domain in eqq0.
           eauto.
-        - Case "NNRCimpLet".
+        - Case "NNRSimpLet".
           apply some_olift in sem.
           destruct sem as [? eqq1 eqq2].
           apply some_lift in eqq1.
@@ -176,77 +176,77 @@ Section NNRCimpSemEval.
           destruct p; try discriminate.
           destruct p.
           invcs eqq2.
-          apply nnrc_imp_expr_sem_eval in eqq1.
+          apply nnrs_imp_expr_sem_eval in eqq1.
           eauto.
-        - Case "NNRCimpLet".
+        - Case "NNRSimpLet".
           invcs sem.
           eauto.
-        - Case "NNRCimpFor".
+        - Case "NNRSimpFor".
           destruct d; try discriminate.
-          apply nnrc_imp_expr_sem_eval in eqq.
+          apply nnrs_imp_expr_sem_eval in eqq.
           econstructor; eauto.
           clear eqq.
           revert σ₁ σ₂ sem.
           induction l; intros σ₁ σ₂ sem; invcs sem; eauto 1.
           repeat destr H0.
           eauto.
-        - Case "NNRCimpIf".
-          apply nnrc_imp_expr_sem_eval in eqq.
+        - Case "NNRSimpIf".
+          apply nnrs_imp_expr_sem_eval in eqq.
           destruct d; try discriminate.
           destruct b; eauto.
-        - Case "NNRCimpEither".
-          apply nnrc_imp_expr_sem_eval in eqq.
+        - Case "NNRSimpEither".
+          apply nnrs_imp_expr_sem_eval in eqq.
           destruct d; try discriminate;
             repeat destr sem; invcs sem; eauto.
       }
   Qed.
 
-  Theorem nnrc_imp_sem_eval σc q d :
-    [ h , σc ⊢ q ⇓ d ] <-> nnrc_imp_eval h σc q = Some d.
+  Theorem nnrs_imp_sem_eval σc q d :
+    [ h , σc ⊢ q ⇓ d ] <-> nnrs_imp_eval h σc q = Some d.
   Proof.
     destruct q.
-    unfold nnrc_imp_eval.
+    unfold nnrs_imp_eval.
     split; intros hyp.
     - invcs hyp.
-      apply nnrc_imp_stmt_sem_eval in H.
+      apply nnrs_imp_stmt_sem_eval in H.
       simpl in H.
       rewrite H; trivial.
     - destr hyp.
       destruct p; try discriminate.
       destruct p.
       invcs hyp.
-      apply nnrc_imp_stmt_sem_eval in eqq.
-      generalize (nnrc_imp_stmt_sem_env_stack eqq).
+      apply nnrs_imp_stmt_sem_eval in eqq.
+      generalize (nnrs_imp_stmt_sem_env_stack eqq).
       simpl; intros eqq2; invcs eqq2.
       symmetry in H1; apply domain_nil in H1; subst.
       constructor; simpl; trivial.
   Qed.
 
-  Theorem nnrc_imp_sem_eval_top σc q d :
-    [ h , (rec_sort σc) ⊢ q ⇓ Some d ] <-> nnrc_imp_eval_top h σc q = Some d.
+  Theorem nnrs_imp_sem_eval_top σc q d :
+    [ h , (rec_sort σc) ⊢ q ⇓ Some d ] <-> nnrs_imp_eval_top h σc q = Some d.
   Proof.
     destruct q.
-    unfold nnrc_imp_eval_top, nnrc_imp_sem_top.
-    rewrite nnrc_imp_sem_eval.
+    unfold nnrs_imp_eval_top, nnrs_imp_sem_top.
+    rewrite nnrs_imp_sem_eval.
     unfold olift.
     match_destr; unfold id; simpl; intuition congruence.
   Qed.
 
   Section Core.
-    Theorem nnrc_imp_core_sem_eval σc q d :
-      [ h , σc ⊢ q ⇓ᶜ d ] <-> nnrc_imp_core_eval h σc q = Some d.
+    Theorem nnrs_imp_core_sem_eval σc q d :
+      [ h , σc ⊢ q ⇓ᶜ d ] <-> nnrs_imp_core_eval h σc q = Some d.
     Proof.
       destruct q; simpl.
-      apply nnrc_imp_sem_eval.
+      apply nnrs_imp_sem_eval.
     Qed.
 
-    Theorem nnrc_imp_core_sem_eval_top σc q d :
-      [ h , (rec_sort σc) ⊢ q ⇓ᶜ Some d ] <-> nnrc_imp_core_eval_top h σc q = Some d.
+    Theorem nnrs_imp_core_sem_eval_top σc q d :
+      [ h , (rec_sort σc) ⊢ q ⇓ᶜ Some d ] <-> nnrs_imp_core_eval_top h σc q = Some d.
     Proof.
       destruct q; simpl.
-      apply nnrc_imp_sem_eval_top.
+      apply nnrs_imp_sem_eval_top.
     Qed.
 
   End Core.
 
-End NNRCimpSemEval.
+End NNRSimpSemEval.
