coq/NNRSimp/Lang/NNRSimpSize.v
@@ -1,0 +1,81 @@
+(*
+ * Copyright 2015-2016 IBM Corporation
+ *
+ * Licensed under the Apache License, Version 2.0 (the "License");
+ * you may not use this file except in compliance with the License.
+ * You may obtain a copy of the License at
+ *
+ * http://www.apache.org/licenses/LICENSE-2.0
+ *
+ * Unless required by applicable law or agreed to in writing, software
+ * distributed under the License is distributed on an "AS IS" BASIS,
+ * WITHOUT WARRANTIES OR CONDITIONS OF ANY KIND, either express or implied.
+ * See the License for the specific language governing permissions and
+ * limitations under the License.
+ *)
+
+Require Import String.
+Require Import Omega.
+Require Import EquivDec.
+Require Import Decidable.
+Require Import Utils.
+Require Import CommonRuntime.
+Require Import NNRSimp.
+
+Section NNRSimpSize.
+
+  Context {fruntime:foreign_runtime}.
+
+  Fixpoint nnrs_imp_expr_size (n:nnrs_imp_expr) : nat
+    := match n with
+       | NNRSimpGetConstant v => 1
+       | NNRSimpVar v => 1
+       | NNRSimpConst d => 1
+       | NNRSimpBinop op n₁ n₂ => S (nnrs_imp_expr_size n₁ + nnrs_imp_expr_size n₂)
+       | NNRSimpUnop op n₁ => S (nnrs_imp_expr_size n₁)
+       | NNRSimpGroupBy g sl e => S (nnrs_imp_expr_size e)
+       end.
+
+    Fixpoint nnrs_imp_stmt_size (n:nnrs_imp_stmt) : nat
+    := match n with
+       | NNRSimpSeq s₁ s₂ => S (nnrs_imp_stmt_size s₁ + nnrs_imp_stmt_size s₂)
+       | NNRSimpAssign _ e => S (nnrs_imp_expr_size e)
+       | NNRSimpLet v None s => S (nnrs_imp_stmt_size s)
+       | NNRSimpLet v (Some e) s => S (nnrs_imp_expr_size e + nnrs_imp_stmt_size s)
+       | NNRSimpFor v n₁ n₂ => S (nnrs_imp_expr_size n₁ + nnrs_imp_stmt_size n₂)
+       | NNRSimpIf n₁ n₂ n₃ => S (nnrs_imp_expr_size n₁ + nnrs_imp_stmt_size n₂ + nnrs_imp_stmt_size n₃)
+       | NNRSimpEither nd vl nl vr nr => S (nnrs_imp_expr_size nd + nnrs_imp_stmt_size nl + nnrs_imp_stmt_size nr)
+       end.
+
+    Definition nnrs_imp_size (q:nnrs_imp) : nat :=
+      let (n, v) := q in
+      nnrs_imp_stmt_size n.
+
+    Lemma nnrs_imp_expr_size_nzero (n:nnrs_imp_expr) : nnrs_imp_expr_size n <> 0.
+    Proof.
+      induction n; simpl; omega.
+    Qed.
+
+    Lemma nnrs_imp_stmt_size_nzero (n:nnrs_imp_stmt) : nnrs_imp_stmt_size n <> 0.
+    Proof.
+      induction n; simpl; try destruct o; try omega.
+    Qed.
+
+    Corollary nnrs_imp_size_nzero (q:nnrs_imp) : nnrs_imp_size q <> 0.
+    Proof.
+      destruct q.
+      apply nnrs_imp_stmt_size_nzero.
+    Qed.
+
+    Section Core.
+      Program Definition nnrs_imp_core_size (q:nnrs_imp_core) : nat
+        := nnrs_imp_size q.
+
+      Lemma nnrs_imp_core_size_nzero (q:nnrs_imp_core) :
+        nnrs_imp_core_size q <> 0.
+      Proof.
+        apply nnrs_imp_size_nzero.
+      Qed.
+    End Core.
+
+End NNRSimpSize.
