coq/NNRSimp/Lang/NNRSimpVars.v
@@ -1,0 +1,66 @@
+(*
+ * Copyright 2015-2016 IBM Corporation
+ *
+ * Licensed under the Apache License, Version 2.0 (the "License");
+ * you may not use this file except in compliance with the License.
+ * You may obtain a copy of the License at
+ *
+ * http://www.apache.org/licenses/LICENSE-2.0
+ *
+ * Unless required by applicable law or agreed to in writing, software
+ * distributed under the License is distributed on an "AS IS" BASIS,
+ * WITHOUT WARRANTIES OR CONDITIONS OF ANY KIND, either express or implied.
+ * See the License for the specific language governing permissions and
+ * limitations under the License.
+ *)
+
+Require Import String.
+Require Import List.
+Require Import Arith.
+Require Import EquivDec.
+Require Import Morphisms.
+Require Import Arith.
+Require Import Max.
+Require Import Bool.
+Require Import Peano_dec.
+Require Import EquivDec.
+Require Import Decidable.
+Require Import Utils.
+Require Import CommonRuntime.
+Require Import NNRSimp.
+
+Section NNRSimpVars.
+
+  Context {fruntime:foreign_runtime}. 
+  Context (h:brand_relation_t).
+  
+  Fixpoint nnrs_imp_expr_free_vars (e:nnrs_imp_expr) : list var
+    := match e with 
+       | NNRSimpGetConstant _ => nil
+       | NNRSimpVar v => v :: nil
+       | NNRSimpConst _ => nil
+       | NNRSimpBinop _ e₁ e₂ => nnrs_imp_expr_free_vars e₁ ++ nnrs_imp_expr_free_vars e₂
+       | NNRSimpUnop _ e₁ => nnrs_imp_expr_free_vars e₁ 
+       | NNRSimpGroupBy _ _ e₁ => nnrs_imp_expr_free_vars e₁
+       end.
+
+    Fixpoint nnrs_imp_stmt_free_vars (s:nnrs_imp_stmt) : list var
+      := match s with
+         | NNRSimpSeq s₁ s₂ =>
+           nnrs_imp_stmt_free_vars s₁ ++ nnrs_imp_stmt_free_vars s₂
+         | NNRSimpAssign v e =>
+           v::(nnrs_imp_expr_free_vars e)
+         | NNRSimpLet v eo s₀ =>
+           match eo with
+           | Some e => nnrs_imp_expr_free_vars e
+           | None => nil
+           end ++ remove string_eqdec v (nnrs_imp_stmt_free_vars s₀)
+         | NNRSimpFor v e s₀ =>
+           nnrs_imp_expr_free_vars e ++ remove string_eqdec v (nnrs_imp_stmt_free_vars s₀)
+         | NNRSimpIf e s₁ s₂ =>
+           nnrs_imp_expr_free_vars e ++ nnrs_imp_stmt_free_vars s₁ ++ nnrs_imp_stmt_free_vars s₂
+         | NNRSimpEither e x₁ s₁ x₂ s₂ =>
+           nnrs_imp_expr_free_vars e ++ remove string_eqdec x₁ (nnrs_imp_stmt_free_vars s₁) ++ remove string_eqdec x₂ (nnrs_imp_stmt_free_vars s₂)
+       end.
+
+End NNRSimpVars.
